ironfleet/src/Dafny/Distributed/Impl/WS/HostModel.i.dfy
@@ -1,0 +1,54 @@
+include "HostState.i.dfy"
+include "PacketParsing.i.dfy"
+
+module SHT__HostModel_i {
+import opened WS__HostState_i
+import opened WS__PacketParsing_i
+
+
+method InitHostState(constants:ConstantsState, me:EndPoint, fs:FileSystemState) returns (host:HostState)
+    requires ConstantsStateIsValid(constants);
+    requires EndPointIsAbstractable(me);
+    requires fs != null;
+    ensures InitHostStatePostconditions(constants, host);
+    ensures host.me == me;
+    ensures host.constants == constants;
+{
+    host := HostState(constants, fs, me, []);
+    
+    assert Host_Init(AbstractifyHostStateToHost(host), fs, AbstractifyEndPointToNodeIdentity(me),  AbstractifyEndPointsToNodeIdentities(constants.hostIds), AbstractifyCParametersToParameters(constants.params));
+}
+
+method IsValidHTTPReqImpl(req:HTTPRequest) returns (isValid:bool, filePath:seq<char>)
+    ensures isValid ==> IsValidHTTPReq(req);
+    ensures isValid ==> IsValidFilePathInHTTPReq(req, filePath);
+
+method FileExists(filePath:seq<char>) returns (b:bool)
+
+method GetFileContents(filePath:seq<char>) returns (contents:seq<byte>)
+
+method HostModelNextGetRequest(host:HostState, cpacket:CPacket) returns (host':HostState, sent_packets:seq<CPacket>)
+    requires NextGetRequestPreconditions(host, cpacket);
+    ensures NextGetRequestPostconditions(host, cpacket, host', sent_packets);
+{
+
+    var req := cpacket.msg.req;
+    var isValid, filePath;
+    isValid, filePath := IsValidHTTPReqImpl(req);
+    var res;
+
+    if (isValid) {
+        assert IsValidHTTPReq(req);
+        var b := FileExists(filePath);
+        if b {
+            var contents := GetFileContents(filePath);
+            res := GetProtocolVersion() + " " + GetHTTPCode("OK") + LineBreaks() + BytesToString(contents);
+        } else {
+            res := GetProtocolVersion() + " " + GetHTTPCode("Not Found");
+        }
+    } else {
+        res := GetProtocolVersion() + " " + GetHTTPCode("Invalid");
+    }
+    assume false;
+}
+}
